thy/Routing/Linux_Router.thy
@@ -1,8 +1,8 @@
 theory Linux_Router
 imports 
 	Routing_Table
-	"../../Simple_Firewall/SimpleFw_Semantics"
-	"../../Simple_Firewall/Simple_Packet"
+	"../Simple_Firewall/SimpleFw_Semantics"
+	"../Simple_Firewall/Simple_Packet"
 	"~~/src/HOL/Library/Monad_Syntax"
 begin
 
